% Formulas for your convinence
\documentclass{article}
\usepackage{latexsym,bm,amsmath,amssymb}
\begin{document}

%%%%%%%%%%%%%%%%%%%%%%%%%%%%%%%%%%%%%%%%%%%%%%%%%%%%%%%%%%%%%%%%%%%%%%%%%%%%%%%%%%%%%%%%%
%%%% Chapter 5

%  Exercise 5.3
\[
  \begin{aligned}
    Q(s, a) &= \mathbb{E}[R_{t+1} + \gamma V(S_{t+1}) | S_t=s, A_t=a]\\
    &=\sum_{s',r} p(s',r|s,a) [r + \gamma V(s')]\\
    &=r(s,a) + \gamma \sum_{s'} p(s'|s,a) \frac {\sum_{t'\in\tau(s')}\rho_{t':T(t')-1}G_{t'}}
                                                {\sum_{t'\in\tau(s')}\rho_{t':T(t')-1}}
  \end{aligned}
\]

%  Exercise 5.5
\[
  \begin{aligned}
    &\text{ For every-visit MC, the expected square of importance-sampling scaled return for a state s is: } \\
    &\qquad \quad\ \mathbb{E}_b[\sum_{t'\in\tau(s)}(\prod_{t=t'}^{T-1} \frac {\pi(A_t|S_t)} {b(A_t|S_t)})^2]\\
    &\qquad \ = \mathbb{E}_b[(\prod_{t=0}^{T-1} \frac {\pi(A_t|S_t)} {b(A_t|S_t)})^2] \ + \
                \mathbb{E}_b[\sum_{t'\in\tau(s), t'\not=0}(\prod_{t=t'}^{T-1} \frac {\pi(A_t|S_t)} {b(A_t|S_t)})^2]\\
    &\qquad >=  \mathbb{E}_b[(\prod_{t=0}^{T-1} \frac {\pi(A_t|S_t)} {b(A_t|S_t)})^2] \ \ \ (1) \\
    &\text{ It is proven that (1) has infinite variance, so the variance for every-visit MC estimator is still infinite.} \\
  \end{aligned}
\]

%  Exercise 5.7
\[
  \begin{aligned}
    V_{n+1} &\overset {.} {=} \frac {\sum_{k=1}^{n} W_k G_k} {\sum_{k=1}^{n} W_k}, \ \ n \geq 1 \\
    &= \frac {\sum_{k=1}^{n-1} W_k G_k + W_nG_n} {\sum_{k=1}^{n} W_k} \\
    &= \frac {\frac {\sum_{k=1}^{n-1} W_k G_k + W_nG_n} {\sum_{k=1}^{n-1} W_k}}
             {\frac {\sum_{k=1}^{n} W_k} {\sum_{k=1}^{n-1} W_k}}\\
    &= \frac {V_n + \frac {W_nG_n} {\sum_{k=1}^{n-1} W_k}}
             {\frac {\sum_{k=1}^{n} W_k} {\sum_{k=1}^{n-1} W_k}}\\
   &= \frac {\sum_{k=1}^{n-1} W_k V_n} {\sum_{k=1}^{n} W_k} + \frac {W_nG_n} {\sum_{k=1}^{n} W_k} \\
   &= \frac {\sum_{k=1}^{n-1} W_k V_n} {\sum_{k=1}^{n} W_k} +
      (\frac {W_n V_n} {\sum_{k=1}^{n} W_k} - \frac {W_n V_n} {\sum_{k=1}^{n} W_k}) +
      \frac {W_nG_n} {\sum_{k=1}^{n} W_k} \\
   &= V_n + \frac {W_n(G_n - V_n)} {\sum_{k=1}^{n} W_k} \\
   &= V_n + \frac {W_n} {C_n}[G_n - V_n], \ \ C_{n+1} \overset {.} {=} C_n + W_{n+1}
  \end{aligned}
\]

\end{document}
